cem.v
@@ -1,27 +1,29 @@
-Require Import expr_db_nat util.
+Require Import db util.
 Require Import Arith.EqNat.
-Require Import List Unicode.Utf8.
+Require Import List Unicode.Utf8 Arith.Peano_dec.
 Require Import CpdtTactics.
 
 Definition append := Datatypes.app.
 
 Inductive closure : Type := 
-  | close : expr → nat → closure. 
+  | close : tm → nat → closure. 
 
 Inductive cell : Type :=
   | cl : closure → nat → cell.
 
+Definition clclose (c: cell) : closure := match c with cl c e => c end.
+
 Definition heap := Map nat cell.
 
 Inductive configuration : Type :=
-  | st : heap → closure → configuration.
+  | conf : heap → closure → configuration.
 
-Definition I (e : expr) : configuration := st nil (close e 0).
+Definition I (e : tm) : configuration := conf nil (close e 0).
 
 Notation " x ↦ M " := (x, M) (at level 40).
-Notation " ⟨ Φ ⟩ m " := (st Φ m) (at level 40).
-Notation " ⟨ Ψ , b ⟩ N " := (st (cons b Ψ) N) (at level 40).
-Notation " ⟨ Φ , b , Ψ ⟩ N " := (st (append _ Ψ (cons b Φ)) N) (at level 40).
+Notation " ⟨ Φ ⟩ m " := (conf Φ m) (at level 40).
+Notation " ⟨ Ψ , b ⟩ N " := (conf (cons b Ψ) N) (at level 40).
+Notation " ⟨ Φ , b , Ψ ⟩ N " := (conf (append _ Ψ (cons b Φ)) N) (at level 40).
 Notation " { M , e } " := (cl M e).
 Notation " < M , e > " := (close M e).
 
@@ -38,36 +40,35 @@ Definition lookup {a} (x:nat) (l:list (nat * a)) : option a :=
     | Some (k,v) => Some v
   end.
 
-Fixpoint clu (v env:nat) (h:heap) : option nat := match v with
-  | 0 => Some env
-  | S n => match lookup env h with
-    | Some (cl c a) => clu n a h
-    | None => None
+Fixpoint clu (v env:nat) (h:heap) : option (nat * closure) := match lookup env h with
+  | None => None
+  | Some (cl c a) => match v with
+    | S n => clu n a h
+    | 0 => Some (env, c)
     end
   end.
 
 Definition fresh (n : nat) (h : heap) := 
   ~ In n (domain h).
 
-Definition closed_under (c : configuration) : Prop := match c with
-  | st h (close t e) => forevery (fvs t) 
-      (λ x, ∃e', cactus_lookup x e h e' ∧ In e' (domain h))
+Definition closed_under (c : closure) (h : heap)  : Prop := match c with
+  | close t e => forevery (fvs t) 
+      (λ x, ∃e' c', clu x e h = Some (e',c') ∧ In e' (domain h))
   end.
 
-Definition closed (t : expr) : Prop := closed_under (st nil (close t 0)).
+Definition closed (t : tm) : Prop := closed_under (close t 0) nil.
 
 Definition well_formed_heap (h : heap) : Prop := forevery h 
-  (λ x, match x with | (v,cl c e) => closed_under (st h c) end). 
+  (λ x, match x with | (v,cl c e') => closed_under c h end). 
 
 Definition well_formed (c : configuration) : Prop := match c with 
-  | st h t => closed_under c ∧ well_formed_heap h 
+  | conf h t => closed_under t h ∧ well_formed_heap h 
   end.
 
 Reserved Notation " c1 '⇓' c2 " (at level 50).
 Inductive step : configuration → configuration → Prop :=
-  | Id : ∀ M B x y z Φ Ψ Υ v e, 
-                  cactus_lookup v z (Υ ++ (x ↦ {M,y} :: Φ)) x →
-              ⟨Φ, (x ↦ {M,y}), Υ⟩M ⇓ ⟨Ψ, (x ↦ {M,y}), Υ⟩close (:λB) e →
+  | Id : ∀ M B x y z Φ Ψ Υ v e, clu v z (Υ ++ x ↦ {M,y} :: Φ) = Some (x, M) → 
+            ⟨Φ, (x ↦ {M,y}), Υ⟩M ⇓ ⟨Ψ, (x ↦ {M,y}), Υ⟩close (:λB) e →
     ⟨Φ, x ↦ {M, y}, Υ⟩close (var v) z ⇓ ⟨Ψ, x ↦ {close (:λB) e, y}, Υ⟩close (:λB) e
   | Abs : ∀ N Φ e, ⟨Φ⟩close (:λN) e ⇓ ⟨Φ⟩close (:λN) e
   | App : ∀ N M B B' Φ Ψ Υ f e ne ae, fresh f Ψ → 
@@ -80,13 +81,25 @@ Definition configuration' := sig well_formed.
 Definition step' (c1 c2: configuration') : Prop := match (c1, c2) with
   | (exist c1 _, exist c2 _) => step c1 c2 end.
 
-Lemma well_formed_inf : ∀ c x c' n  Φ Υ, well_formed (⟨Φ, x ↦ cl c' n, Υ⟩c) → 
+Lemma well_formed_inf : ∀ c x c' n  Φ Υ, 
+  well_formed (⟨Φ, x ↦ cl c' n, Υ⟩c) → 
   well_formed (⟨Φ, x ↦ cl c' n, Υ⟩c').
   intros. split. inversion H. unfold well_formed_heap in H1. apply forevery_app in H1.
   destruct H1. simpl in H2. destruct H2. auto. 
   auto. inversion H. auto. Qed. 
 
 (*
+Lemma well_formed_inf' : ∀ Φ Ψ x c c' n,
+  well_formed (⟨Φ, x ↦ cl c' n, Ψ⟩c) →
+  well_formed (⟨Φ, x ↦ cl c n, Ψ⟩c).
+intros. split.  inversion H. apply forevery_app in H1. destruct H1. unfold
+closed_under. destruct c. unfold closed_under in H0. simpl in H2. destruct H2. 
+unfold closed_under. rewrite forevery_app.  with (m:=n) (m':=n). assumption.
+unfold well_formed_heap. unfold closed_under.  unfold well_formed_heap in H0.
+unfold closed_under in H0. rewrite domain_inf with (m:=N) (m':=M). rewrite
+forevery_app. rewrite forevery_app in H0. destruct H0. split. crush. crush. 
+Qed.
+
 TODO
 Lemma cactus_lookup_inf : ∀ v x y m n e Φ Υ, cactus_lookup v x (Φ ++ (y ↦ {m, n}) :: Υ) e → ∀ M, cactus_lookup v x (Φ ++ (y ↦ {M, n}) :: Υ) e.
 intros. 
@@ -103,7 +116,6 @@ Lemma inf_well_formed : ∀ c x c' n  Φ Υ, well_formed (⟨Φ, x ↦ cl c' n, 
 
 Theorem well_formed_step : ∀ c v, well_formed c → c ⇓ v → well_formed v.
 intros. induction H0. apply well_formed_inf in H. apply IHstep in H.  
-*)
 
 Lemma values_only : ∀ c e M Ψ, c ⇓ ⟨Ψ⟩close M e → value M.
 intros. inversion H; simpl; auto. Qed.
@@ -119,4 +131,4 @@ apply zero.
 apply Abs. 
 Qed.
 
-
+*)
