cesm.v
@@ -2,61 +2,20 @@ Require Import Arith.EqNat.
 Require Import List Unicode.Utf8.
 Require Import Arith.Peano_dec.
 Require Import CpdtTactics.
-Require Import expr_db_nat util.
-
-Definition append := Datatypes.app.
-
-Inductive closure : Type := 
-  | close : expr → nat → closure. 
-
-Inductive cell : Type :=
-  | cl : closure → nat → cell.
-
-Definition heap := list (nat * cell).
+Require Import db util.
+Require Import cem.
 
 Definition stack := list (closure + nat).
 
-Inductive configuration : Type :=
-  | conf : heap → stack → closure → configuration.
+Inductive state : Type :=
+  | st : heap → stack → closure → state.
 
-Definition I (e : expr) : configuration := conf nil nil (close e 0).
+Definition I (e : tm) : state := st nil nil (close e 0).
 
 Notation " x ↦ M " := (x, M) (at level 40).
-Notation " ⟨ Φ ⟩ m " := (conf Φ m) (at level 40).
-Notation " ⟨ Ψ , b ⟩ N " :=  (conf (cons b Ψ) N) (at level 40).
-Notation " ⟨ Φ , b , Ψ ⟩ N " := (conf (append _ Ψ (cons b Φ)) N) (at level 40).
+Notation " [ Φ , s ] m " := (st Φ s m) (at level 40).
 
-Fixpoint clu (v env:nat) (h:heap) : option (nat * closure) := match lookup eq_nat_dec env h with
-    | Some (cl c env') => match v with 
-      | 0 => Some (env, c) 
-      | S n => clu n env' h
-      end
-    | None => None
-  end.
-
-Definition fresh (n : nat) (h : heap) := 
-  ~ In n (domain h).
-
-Definition c_hp (c : configuration) := match c with
-  | conf h s c => h end.
-
-Axiom new : ∀ (c : configuration), nat.
-Axiom new_fresh : ∀ c, fresh (new c) (c_hp c).
-
-Inductive cactus_lookup : nat → nat → heap → nat → Prop :=
-  | zero : forall x Φ M Υ, cactus_lookup 0 x (append _ Φ (cons (x ↦ M) Υ)) x
-  | pred : forall x y z Φ M Υ i, cactus_lookup i x Φ z → 
-            cactus_lookup (S i) y (append _ Φ (cons (y ↦ (cl M x)) Υ)) z.
-
-Definition closed_under (c : closure) (h : heap) : Prop := match c with
-  | close t e => forevery (fvs t) 
-      (λ x, ∃e', cactus_lookup x e h e' ∧ In e' (domain h))
-  end.
-
-Definition closed (t : expr) : Prop := closed_under (close t 0) nil. 
-
-Definition well_formed_heap (h : heap) : Prop := forevery h 
-  (λ x, match x with | (v,cl c e) => closed_under c h end). 
+Definition closed (t : tm) : Prop := closed_under (close t 0) nil. 
 
 Fixpoint lefts {a b} (l : list (a + b)) : list a := match l with
   | nil => nil
@@ -64,14 +23,28 @@ Fixpoint lefts {a b} (l : list (a + b)) : list a := match l with
   | cons (inr b) t => lefts t
   end.
 
-Definition well_formed (conf : configuration) : Prop := match conf with 
-  | conf h s c => closed_under c h ∧ well_formed_heap h ∧ forevery (lefts s) (flip closed_under h)
+Definition well_formed (st : state) : Prop := match st with 
+  | st h s c => closed_under c h ∧ well_formed_heap h ∧ forevery (lefts s) (flip closed_under h)
   end.
 
 Definition replaceClosure (l:nat) (c:closure) : nat * cell → nat * cell := 
   fun x => match x with
     | (l', cl c' e) => if eq_nat_dec l l' then (l, cl c e) else x
     end.
+
+Reserved Notation " c1 '→_s' c2 " (at level 50).
+Inductive step' : state → state → Prop :=
+  | Upd : ∀ Φ Υ b e e' c l s, 
+  st (Φ++(l,(cl c e'))::Υ) (inr l::s) (close (lam b) e) →_s 
+  st (Φ++(l,(cl (close (lam b) e) e'))::Υ) s (close (lam b) e)
+  | Var : ∀ Φ s v l c e, clu v e Φ = Some (l,c) → 
+  st Φ s (close (var v) e) →_s st Φ (inr l::s) c
+  | Abs : ∀ Φ b e f c s, fresh f Φ → 
+  st Φ (inl c::s) (close (lam b) e) →_s st ((f, cl c e):: Φ) s (close b f)
+  | App : ∀ Φ e s n m, 
+  st Φ s (close (app m n) e) →_s st Φ (inl (close n e)::s) (close m e)
+where " c1 '→_s' c2 " := (step' c1 c2).
+
 
 (* Step as a function *
 
