db.v
@@ -1,62 +1,61 @@
 Require Import Unicode.Utf8.
 Require Import Decidable.
-Require expr expr_db_nat.
+Require expr.
 Require Import List Datatypes util.
 Require Import FunctionalExtensionality CpdtTactics. 
 Require Import Arith.Peano_dec.
 Require Import Program.Basics.
 Set Implicit Arguments.
 
-(* db.v : used to relate debruijn terms with standard terms *) 
-Definition fmap' {A B C} (f : A -> C) : A * B -> C * B  := fun x => match x with
-  | (a, b) => (f a, b) end. 
+Inductive tm : Type := 
+  | var : nat -> tm 
+  | lam : tm -> tm
+  | app : tm -> tm -> tm.
 
-(* a relation between standard lambda terms and deBruijn-indexed term, note that
-  standard variables are nats as well *)
-Fixpoint db (tm : expr.tm) (env : Map nat nat) : option expr_db_nat.expr := match tm with 
-  | expr.var v => match lookup eq_nat_dec v env with
-    | Some v' => Some (expr_db_nat.var v')
-    | None => None
-    end
-  | expr.abs v b => match db b ((v, 0):: map (fmap S) env) with 
-    | Some b' => Some (expr_db_nat.lam b')
-    | None => None
-    end
-  | expr.app m n => match db m env with
-    | Some m' => match db n env with 
-      | Some n' => Some (expr_db_nat.app m' n')
-      | None => None
-      end
-    | None => None
-    end
+Definition value (t : tm) : Prop := match t with
+  | lam _ => True
+  | _ => False
   end.
+
+Fixpoint fvs (e:tm) : list nat := match e with
+  | var v =>  v::nil
+  | lam b =>  map pred (remove 0 (fvs b))
+  | app m n => fvs m ++ fvs n
+  end.
+
+Definition closed (e:tm) := fvs e = nil.
+
+Notation " :λ N " := (lam N) (at level 20).
+Notation " M @ N " := (app M N) (at level 60). 
+Coercion var : nat >-> tm.
+
+Example term_1 : tm := lam (var 0).
+Example term_2 : tm := app term_1 term_1.
 
 (* TODO
 Lemma dbClosedUnder (tm : expr.tm) (env : Map nat nat) : 
   subset (expr.fvs tm) (domain env) → exists e, db tm env = Some e.
 intros. induction tm. apply subset_domain_map with (l:=(expr.fvs (expr.var n)))
 (eq0:=eq_nat_dec) in H. simpl in H. simpl. destruct H. destruct H. rewrite H.
-apply ex_intro with (expr_db_nat.var x). reflexivity. simpl in H. rewrite
+apply ex_intro with (var x). reflexivity. simpl in H. rewrite
 app_subset_and in H. destruct H. apply IHtm1 in H. apply IHtm2 in H0. simpl.
-destruct H, H0. rewrite H. rewrite H0. apply ex_intro with (expr_db_nat.app x
+destruct H, H0. rewrite H. rewrite H0. apply ex_intro with (app x
 x0). reflexivity. simpl in H. simpl. rewrite <- subset_remove_cons in H. 
 rewrite <- domain_fmap with (C:=nat) (f:=S) in H. 
 induction (expr.fvs tm).
 assert (subset nil (domain env)). apply subset_nil. apply IHtm in H0. destruct
-H0. apply ex_intro with (expr_db_nat.lam x). 
+H0. apply ex_intro with (lam x). 
 *)
-
-Definition alpha_equiv (t1 t2 : expr.tm) : Prop := db t1 = db t2.
 
 (*
 Theorem closed_db_under : forall f t, subset (expr.fvs t) (domain f) -> exists
 e, db t f e.
 intros. induction t. destruct H. apply in_split in H. crush. clear H0.
-apply ex_intro with (expr_db_nat.var n).
+apply ex_intro with (var n).
 induction f. crush. induction t. inversion H. inversion H0. unfold expr.fvs
 in H. apply app_subset_and in H. destruct H. crush. apply ex_intro with
-(expr_db_nat.app x0 x). apply dbApp; assumption. apply ex_intro with
-expr_db_nat.lam 
+(app x0 x). apply dbApp; assumption. apply ex_intro with
+lam 
 induction e. crush. apply in_split in H0. destruct H0. destruct H.   
 induction H. crush. unfold domain. rewrite map_app. rewrite in_app_iff.
 right. crush. crush. rewrite <- subset_remove_cons. rewrite domain_fmap in IHdb.
