cem_cesm.v
@@ -1,0 +1,54 @@
+Require Import cem cesm.
+Require Import Unicode.Utf8.
+Require Import relations. 
+Require Import List. 
+
+Notation " c1 '→_s*' c2 " := (refl_trans_clos step' c1 c2) (at level 30). 
+
+Definition b2s (c : configuration) : stack → state := match c with
+  | conf h c => λ s, st h s c end.
+
+Definition convert_to_cesm (c c' : configuration) : Prop := match (c, c') with
+  | (conf h c, conf h' c') => ∀ s, (st h s c) →_s* (st h' s c') end.
+
+Lemma cem_cesm : ∀ c v, c ⇓ v → ∀ s, b2s c s →_s* b2s v s. 
+(* Var *)
+intros c v H. induction H. simpl. simpl in IHstep. 
+assert (∀ s, step' (st (Υ ++ (x ↦ {M,y} :: Φ)) s (close (db.var v) z)) 
+                   (st (Υ ++ (x ↦ {M,y} :: Φ)) (inr x::s) M)).
+intros. apply Var. assumption. 
+assert (∀ s, step' (st (Υ ++ x ↦ {M, y} :: Ψ) (inr x :: s) (close (db.lam B) e))
+                   (st (Υ ++ x ↦ {close (db.lam B) e, y} :: Ψ) s (close (db.lam B) e)))
+.
+apply Upd. 
+intros. rename y into Y.  
+apply t_step with (y:=[Υ ++ x ↦ {M, Y} :: Φ, inr x :: s]M). auto. 
+apply t_step2 with (y:= [Υ ++ x ↦ {M, Y} :: Ψ, inr x :: s](close (db.lam B) e)). 
+auto. auto.   
+(* Lam *)
+intros. apply t_refl. 
+(* App *)
+intros. apply t_step with (y:=b2s (⟨Φ ⟩ close M e) (inl (close N e)::s)). 
+apply App. 
+apply refl_trans_clos_app with (y:=b2s (⟨Ψ, f ↦ {close N e, ne} ⟩ close B f) s).
+apply t_step2 with (y:=b2s (⟨Ψ ⟩ close (db.lam B) ne) (inl (close N e):: s)).
+simpl. rename e into E. rename s into S. apply Abs with (b:=B) (e:=ne)
+(c:=close N E) (s:= S) in H.  
+assumption.
+auto. 
+auto. 
+Qed. 
+
+Definition s2b (s : state) : configuration := match s with
+  | st h s c => conf h c
+  end.
+
+Definition st_stack := λ s, match s with
+  | st h s c => s
+  end.
+
+
+(*
+Lemma cesm_cem : ∀ c c' v, c →_s c' → c' →_s* v → st_stack c = st_stack v → s2b c ⇓ s2b v.
+intros. induction H0. induction H. simpl in H1. inversion v. induction H1. 
+*)
