compiler.v
@@ -1,13 +1,12 @@
-Require expr expr_db_nat cbn cem cesm.
-Require Import db util assembly.
-Require Import Arith.Peano_dec.
-Require Import List Datatypes.
+Require expr cbn cem cesm im db assembly.
+Require cbn_cem cem_cesm.
 Require Import Unicode.Utf8.
+Require Import util expr_db db_assembly.
 
 (* This file has the high level structure of the compiler and the corresponding
 main theorems of correctness *)
 
-Definition compile (t : expr.tm) : option Program := match db t nil with
+Definition compile (t : expr.tm) : option assembly.Program := match db t nil with
   | Some a => Some (assemble a)
   | None => None 
   end.
