db_assembly.v
@@ -1,0 +1,6 @@
+Require Import db assembly util.
+
+(* Assembles deBruijn indices to instructions *)
+Fixpoint assemble (t : tm) : Program.
+Admitted.
+  
