im.v
@@ -1,0 +1,13 @@
+(* Instruction Machine *)
+
+Require Import assembly util.
+Require Import Unicode.Utf8.
+
+Definition Heap := Map Ptr Word.
+Definition RegisterFile := Reg → Word.
+
+Inductive State := 
+  | st : RegisterFile → Program → Stack → Heap → State.
+
+Definition I (p : Program) : State := st (λ _, 0) p nil nil. 
+
